Lib/DerivationTests.v
@@ -5,17 +5,17 @@ Open Scope string_scope.
 
 (* Manual proof of a derivation (don't do this again) *)
 Example derivesTest1 :
-  (@derivesTree g311) (NT "S") g311Sentence1 g311ParseTree1.
+  (@derivesTree g311) (NT X) g311Sentence1 g311ParseTree1.
 Proof.
   apply derivesNT with 
-      (x := "S")
-      (gamma := [T "if" ; NT "E" ; T "then" ; NT "S" ; T "else" ; NT "S"]).
+      (x := X)
+      (gamma := [T "if" ; NT E ; T "then" ; NT X ; T "else" ; NT X]).
   - left. reflexivity.
   - apply derivesCons with (prefix := ["if"]).
     + apply derivesT.
     + apply derivesCons with (prefix := ["num" ; "==" ; "num"]).
       * apply derivesNT with 
-            (x := "E")
+            (x := E)
             (gamma := [T "num" ; T "==" ; T "num"]).
         { repeat (try (left ; reflexivity) ; right). }
         { apply derivesCons with (prefix := ["num"]).
@@ -29,14 +29,14 @@ Proof.
         { apply derivesT. }
         apply derivesCons with (prefix := ["print" ; "num" ; "==" ; "num"]).
         { apply derivesNT with 
-              (x := "S")
-              (gamma := [T "print" ; NT "E"]).
+              (x := X)
+              (gamma := [T "print" ; NT E]).
           { repeat (try (left ; reflexivity) ; right). }
           apply derivesCons with (prefix := ["print"]).
           { apply derivesT. }
           apply derivesCons with (prefix := ["num" ; "==" ; "num"]).
           { apply derivesNT with
-                (x := "E") 
+                (x := E) 
                 (gamma := [T "num" ; T "==" ; T "num"]).
             { repeat (try (left ; reflexivity) ; right). }
             apply derivesCons with (prefix := ["num"]).
@@ -51,14 +51,14 @@ Proof.
         { apply derivesT. }
         apply derivesCons with (prefix := ["print" ; "num" ; "==" ; "num"]).
         { apply derivesNT with 
-              (x := "S")
-              (gamma := [T "print" ; NT "E"]).
+              (x := X)
+              (gamma := [T "print" ; NT E]).
           { repeat (try (left ; reflexivity) ; right). }
           apply derivesCons with (prefix := ["print"]).
           { apply derivesT. }
           apply derivesCons with (prefix := ["num" ; "==" ; "num"]).
           { apply derivesNT with 
-                (x := "E")
+                (x := E)
                 (gamma := [T "num" ; T "==" ; T "num"]).
             { repeat (try (left ; reflexivity) ; right). }
             apply derivesCons with (prefix := ["num"]).
@@ -74,34 +74,34 @@ Qed.
 
 (* A (slightly) more automated proof of the same derivation. *)
 Example derivesTest2 :
-  (@derivesTree g311) (NT "S") g311Sentence1 g311ParseTree1.
+  (@derivesTree g311) (NT X) g311Sentence1 g311ParseTree1.
 Proof.
   apply derivesNT with 
-      (x := "S")
-      (gamma := [T "if" ; NT "E" ; T "then" ; NT "S" ; T "else" ; NT "S"]);
+      (x := X)
+      (gamma := [T "if" ; NT E ; T "then" ; NT X ; T "else" ; NT X]);
     derCrush.
   apply derivesCons with (prefix := ["num" ; "==" ; "num"]).
   - apply derivesNT with 
-        (x := "E")
+        (x := E)
         (gamma := [T "num" ; T "==" ; T "num"]); derCrush.
   - derCrush.
     apply derivesCons with (prefix := ["print" ; "num" ; "==" ; "num"]).
     + apply derivesNT with 
-          (x := "S")
-          (gamma := [T "print" ; NT "E"]); derCrush.
+          (x := X)
+          (gamma := [T "print" ; NT E]); derCrush.
       apply derivesCons with (prefix := ["num" ; "==" ; "num"]).
       * apply derivesNT with 
-            (x := "E")
+            (x := E)
             (gamma := [T "num" ; T "==" ; T "num"]); derCrush.
       * derCrush.
     + derCrush.
       apply derivesCons with (prefix := ["print" ; "num" ; "==" ; "num"]).
       * apply derivesNT with 
-            (x := "S")
-            (gamma := [T "print" ; NT "E"]); derCrush.
+            (x := X)
+            (gamma := [T "print" ; NT E]); derCrush.
         apply derivesCons with (prefix := ["num"; "=="; "num"]).
         { apply derivesNT with 
-              (x := "E")
+              (x := E)
               (gamma := [T "num" ; T "==" ; T "num"]); derCrush. }
         derCrush.
       * derCrush.
